Move some reusable code to TODO.v

coq/def/TODO.v
@@ -275,3 +275,133 @@ Ltac des_sumbool :=
     | [ H: proj_sumbool ?x = false |- _ ] => apply proj_sumbool_false in H
     end.
 (* check InvBooleans tactic in compcert *)
+
+(* It is important that f does not look into A *)
+(* This can give you following spec *)
+Fixpoint filter_AL_atom {A: Type} (f: atom -> bool) (al: AssocList A) :=
+  match al with
+  | [] => []
+  | (a, h) :: t =>
+    if f(a)
+    then (a, h) :: (filter_AL_atom f t)
+    else (filter_AL_atom f t)
+  end.
+
+Lemma lookup_AL_filter_false {A: Type} id al f
+      (NOPASS: f id = false):
+  <<NORESULT: lookupAL A (filter_AL_atom f al) id = None>>.
+Proof.
+  red.
+  induction al; ss.
+  destruct a; ss.
+  destruct (f a) eqn:T; ss.
+  destruct (id == a) eqn:T2; ss. subst.
+  clarify.
+Qed.
+
+Lemma lookup_AL_filter_true {A: Type} id al f
+      (PASS: f id = true):
+  <<RESULT: lookupAL A (filter_AL_atom f al) id =
+              lookupAL A al id >>.
+Proof.
+  red.
+  induction al; ss.
+  destruct a.
+  destruct (id == a) eqn:T; ss.
+  - subst. rewrite PASS. ss. rewrite T. ss.
+  - destruct (f a) eqn:T2; ss.
+    rewrite T. ss.
+Qed.
+
+Lemma lookup_AL_filter_some {A: Type} id val al f
+  (FILTERED: lookupAL A (filter_AL_atom f al) id = Some val):
+  lookupAL A al id = Some val.
+Proof.
+  destruct (f id) eqn:T.
+  - exploit (@lookup_AL_filter_true A); eauto. ii; des.
+    rewrite FILTERED in x0. ss.
+  - exploit (@lookup_AL_filter_false A); eauto. ii; des.
+    rewrite FILTERED in x0. ss.
+Qed.
+
+Lemma in_filter_find {A: Type} (x: A) f l
+  (IN: In x (filter f l)):
+  exists x2, find f l = Some x2 /\ f x2.
+Proof.
+  induction l; ss.
+  destruct (f a) eqn:T.
+  - eexists; eauto.
+  - clear T. specialize (IHl IN). ss.
+Qed.
+
+Lemma In_concat {A B C: Type} f (a: A) (x: B) xs
+      (IN1: In a (f x))
+      (IN2: In (f x) (List.map f xs)):
+  <<IN3: In a (concat (List.map f xs))>>.
+Proof.
+  red.
+  generalize dependent a.
+  generalize dependent x.
+  induction xs; ii; ss.
+  des.
+  - rewrite IN2.
+    destruct (f x); inv IN1.
+    + ss. left. ss.
+    + ss. right.
+      eapply in_or_app.
+      left; ss.
+  - exploit IHxs; eauto; []; ii; des.
+    destruct (f a) eqn:T; ss.
+    right.
+    eapply in_or_app. right. ss.
+Qed.
+
+Lemma In_map {A B: Type} (f: A -> B) (a: A) al
+      (IN: In a al):
+        <<IN2: In (f a) (List.map f al)>>.
+Proof.
+  generalize dependent a.
+  induction al; ii; ss.
+  des; red; ss. subst.
+  - left; ss.
+  - right. eapply IHal; ss.
+Qed.
+
+Lemma forallb_filter_map {A B: Type} (f: B -> bool) (g: A -> option B) (xs: list A)
+      (FORALL: List.forallb f (filter_map g xs)):
+  (* List.forallb (fun x => match (g x) with | Some y => f y | None => true end) xs. *)
+  <<FORALL: List.forallb (fun x => List.forallb f (g x)) xs>>.
+Proof.
+  red.
+  generalize dependent FORALL.
+  induction xs; ii; ss.
+  destruct (g a) eqn:T; des_bool; ss.
+  - unfold is_true in FORALL. (* des_bool should solve this!!! KILL ALL is_true *)
+    repeat (des_bool; des).
+    rewrite FORALL.
+    rewrite IHxs; eauto.
+  - rewrite IHxs; ss.
+Qed.
+
+Lemma find_app
+      A pred (l1 l2:list A):
+  find pred (l1 ++ l2) =
+  match find pred l1 with
+  | Some v1 => Some v1
+  | None => find pred l2
+  end.
+Proof.
+  induction l1; ss. destruct (pred a); ss.
+Qed.
+
+Lemma In_eq_find {X} (x: X) xs (x_eq_dec: forall x1 x2, {x1 = x2} + {x1 <> x2})
+      (IN: In x xs):
+  <<FOUND: (find (fun y => x_eq_dec x y) xs)>>.
+Proof.
+  red.
+  generalize dependent IN.
+  induction xs; ii; inv IN; ss.
+  - destruct (x_eq_dec x x) eqn:T; ss.
+  - specialize (IHxs H).
+    destruct (x_eq_dec x a) eqn:T; ss.
+Qed.
